HarderNarasimhan/JordanHolderFiltration/Defs.lean
@@ -1,4 +1,6 @@
 import HarderNarasimhan.NashEquilibrium.Impl
+import HarderNarasimhan.FirstMoverAdvantage.Results
+import HarderNarasimhan.SlopeLike.Result
 import Mathlib.Order.OrderIsoNat
 open Classical
 
@@ -31,6 +33,7 @@ where
   step_cond₂ : ∀ i : ℕ, (hi : i < Nat.find fin_len) →
     ∀ z : ℒ, (h' : filtration (i+1) < z) → (h'' : z < filtration i) →
     μ ⟨(filtration (i+1), z), h'⟩ < μ ⟨(filtration (i+1), filtration i), strict_anti i (i+1) (lt_add_one i) hi⟩
+
 
 
 instance {ℒ : Type*} [Nontrivial ℒ] [Lattice ℒ] [BoundedOrder ℒ]
@@ -85,5 +88,153 @@ instance {ℒ : Type*} [Nontrivial ℒ] [Lattice ℒ] [BoundedOrder ℒ] [WellFo
     apply le_sSup
     use x, ⟨in_TotIntvl x, Ne.symm <| bot_lt_iff_ne_bot.1 hx⟩
   exact (not_le_of_lt <| h ▸ lt_top_iff_ne_top.2 hftp.fin_tot_payoff) this_q
+
+lemma fuck {ℒ : Type*} [Nontrivial ℒ] [Lattice ℒ] [BoundedOrder ℒ] [WellFoundedGT ℒ]
+{S : Type*} [CompleteLinearOrder S]
+(μ : {p : ℒ × ℒ // p.1 < p.2} → S) [SlopeLike μ] [sdc : StrongDescendingChainCondition' μ]
+(filtration : ℕ → ℒ) (fin_len : ∃ N : ℕ, filtration N =⊥)
+(strict_anti : ∀ i j : ℕ, i < j → j ≤ Nat.find (fin_len) → filtration j < filtration i)
+(step_cond₁ : ∀ k : ℕ,  (hk : k < Nat.find (fin_len)) → μ ⟨(filtration (k + 1),filtration k),strict_anti k (k+1) (lt_add_one k) hk⟩ = μ ⟨(⊥,⊤),bot_lt_top⟩) :
+(∀ i : ℕ, (hi : i < Nat.find fin_len) →
+    ∀ z : ℒ, (h' : filtration (i+1) < z) → (h'' : z < filtration i) →
+    μ ⟨(filtration (i+1), z), h'⟩ < μ ⟨(filtration (i+1), filtration i), strict_anti i (i+1) (lt_add_one i) hi⟩)
+↔ (
+∀ i : ℕ, (hi : i < Nat.find fin_len) → Stable (Resμ ⟨(filtration (i+1), filtration i), strict_anti i (i+1) (lt_add_one i) hi⟩ μ)
+) := by
+  constructor
+  · intro h
+    intro i hi
+    have h := h i hi
+    refine { toSemistable := ?_, stable := ?_ }
+    · apply (impl.thm4d21 (Resμ ⟨(filtration (i+1), filtration i), strict_anti i (i+1) (lt_add_one i) hi⟩ μ) inferInstance inferInstance inferInstance).2.2 (fun _ _ ↦ inferInstance)
+      apply (List.TFAE.out (impl.thm4d21 (Resμ ⟨(filtration (i+1), filtration i), strict_anti i (i+1) (lt_add_one i) hi⟩ μ) inferInstance inferInstance inferInstance).1 1 3).1
+      --simp only [μmin_res_intvl,μ_res_intvl]
+      apply eq_of_le_of_le ?_ ?_
+      · apply sInf_le
+        simp only [ne_eq, Set.mem_setOf_eq]
+        use ⊥
+        simp only [bot_ne_top, not_false_eq_true, and_true, exists_prop,in_TotIntvl]
+      · apply le_sInf
+        intro b hb
+        simp only [ne_eq, Set.mem_setOf_eq] at hb
+        rcases hb with ⟨u,hu1,hu2⟩
+        rw [← hu2]
+        simp only [μ_res_intvl]
+        if hu : u = ⊥ then
+          simp only [hu, le_refl]
+        else
+        have h := h u.val (lt_of_le_of_ne u.prop.1 (by
+          by_contra hc
+          refine hu ?_
+          apply Subtype.coe_inj.1
+          exact id (Eq.symm hc)
+          )) (lt_of_le_of_ne u.prop.2 (by
+            by_contra hc
+            refine hu1.2 ?_
+            apply Subtype.coe_inj.1
+            exact hc
+            ))
+        have := ((seesaw_useful μ inferInstance (filtration (i + 1)) u.val (filtration i) ⟨(lt_of_le_of_ne u.prop.1 (by
+          by_contra hc
+          refine hu ?_
+          apply Subtype.coe_inj.1
+          exact id (Eq.symm hc)
+          )),(lt_of_le_of_ne u.prop.2 (by
+            by_contra hc
+            refine hu1.2 ?_
+            apply Subtype.coe_inj.1
+            exact hc
+            ))⟩).1.1 h).2
+        apply le_of_lt this
+    · intro x hx hx'
+      have := (proposition_4_1 (Resμ ⟨(filtration (i+1), filtration i), strict_anti i (i+1) (lt_add_one i) hi⟩ μ) inferInstance inferInstance).1
+      have this' := (proposition_4_1 (Resμ ⟨(filtration (i+1), x.val), (lt_of_le_of_ne x.prop.1 (by
+          by_contra hc
+          refine hx ?_
+          apply Subtype.coe_inj.1
+          exact id (Eq.symm hc)
+          ))⟩ μ) inferInstance inferInstance).1
+      unfold μAstar at this
+      unfold μAstar at this'
+      simp only [μA_res_intvl,μmin_res_intvl] at *
+      rw [this]
+      have t1: @Bot.bot (Interval ⟨(filtration (i + 1), filtration i), strict_anti i (i + 1) (lt_add_one i) hi⟩) OrderBot.toBot = filtration (i + 1) := by rfl
+      simp only [t1] at *
+      have t2 : @Top.top (Interval ⟨(filtration (i + 1), ↑x), lt_of_le_of_ne (Subtype.prop x).left fun hc ↦ hx (Subtype.coe_inj.mp (id (Eq.symm hc)))⟩) OrderTop.toTop = x.val := by rfl
+      simp only [t2] at *
+      have t3 : (@Bot.bot (Interval ⟨(filtration (i + 1), ↑x), lt_of_le_of_ne (Subtype.prop x).left fun hc ↦ hx (Subtype.coe_inj.mp (id (Eq.symm hc)))⟩) OrderBot.toBot).val = filtration (i + 1) := by rfl
+      simp only [t3] at *
+      rw [this']
+      have hss : Semistable (Resμ ⟨(filtration (i + 1), filtration i), strict_anti i (i + 1) (lt_add_one i) hi⟩ μ) := by sorry
+      have := (impl.thm4d21 (Resμ ⟨(filtration (i + 1), filtration i), strict_anti i (i + 1) (lt_add_one i) hi⟩ μ) inferInstance inferInstance inferInstance).2.1 hss
+      have := (List.TFAE.out (impl.thm4d21 (Resμ ⟨(filtration (i + 1), filtration i), strict_anti i (i + 1) (lt_add_one i) hi⟩ μ) inferInstance inferInstance inferInstance).1 1 3).2 this
+      simp only [μmin_res_intvl,μ_res_intvl] at this
+      have t4 : @Bot.bot (Interval ⟨(filtration (i + 1), filtration i), strict_anti i (i + 1) (lt_add_one i) hi⟩) OrderBot.toBot = filtration (i+1) := by rfl
+      simp only [t4] at *
+      have t5 : @Top.top (Interval ⟨(filtration (i + 1), filtration i), strict_anti i (i + 1) (lt_add_one i) hi⟩) OrderTop.toTop = filtration i := by rfl
+      simp only [t5] at *
+      rw [this]
+      apply ne_of_lt
+      have : μmin μ ⟨(filtration (i + 1), ↑x), (lt_of_le_of_ne x.prop.1 (by
+          by_contra hc
+          refine hx ?_
+          apply Subtype.coe_inj.1
+          exact id (Eq.symm hc)
+          ))⟩ ≤ μ ⟨(filtration (i + 1), ↑x), (lt_of_le_of_ne x.prop.1 (by
+          by_contra hc
+          refine hx ?_
+          apply Subtype.coe_inj.1
+          exact id (Eq.symm hc)
+          ))⟩ := by
+        apply sInf_le
+        simp only [ne_eq, id_eq, Set.mem_setOf_eq]
+        use filtration (i + 1)
+        simp only [exists_prop, and_true]
+        constructor
+        · exact ⟨le_rfl,x.prop.1⟩
+        · by_contra hc
+          refine hx ?_
+          apply Subtype.coe_inj.1
+          rw [← hc]
+          rfl
+      refine lt_of_le_of_lt this ?_
+      refine h x.val (lt_of_le_of_ne x.prop.1 (by
+          by_contra hc
+          refine hx ?_
+          apply Subtype.coe_inj.1
+          exact id (Eq.symm hc)
+          )) ?_
+      apply lt_top_iff_ne_top.2 at hx'
+      exact lt_iff_le_not_le.mpr hx'
+  · intro h
+    intro i hi z hz1 hz2
+    have h := h i hi
+    have h1 := h.toSemistable.semistable ⟨z,⟨le_of_lt hz1,le_of_lt hz2⟩⟩ (by
+      by_contra hc
+      apply Subtype.coe_inj.2 at hc
+      simp only at hc
+      rw [hc] at hz1
+      exact lt_irrefl _ hz1
+      )
+    simp only [gt_iff_lt, not_lt] at h1
+    have h2 := h.stable ⟨z,⟨le_of_lt hz1,le_of_lt hz2⟩⟩ (by
+      by_contra hc
+      apply Subtype.coe_inj.2 at hc
+      simp only at hc
+      rw [hc] at hz1
+      exact lt_irrefl _ hz1
+      ) (by
+      by_contra hc
+      apply Subtype.coe_inj.2 at hc
+      simp only at hc
+      rw [hc] at hz2
+      exact lt_irrefl _ hz2
+      )
+    have h' := lt_of_le_of_ne h1 h2
+    simp only [μA_res_intvl] at h'
+
+    sorry
+
+
 
 end HarderNarasimhan
